DS: adapted messages for verification and added events to first two proto. steps
- adapted messages to include plain certificates in order to make verification
of signed certificates possible in DY*
- in the course of the above: splitted sign values from enc. values to allow for
encryption of the concatenation of the plain comm. key and the signed comm.
key and timestamp
- added events to first two protocol steps
- implemented event and sign predicates in DS.Sessions.fsti and DS.Messages.fsti,
respectively (not final)

denning-sacco/DS.Messages.fsti
@@ -19,20 +19,38 @@ let event_send_key (a b srv:principal) (pk_a pk_b ck:bytes) (t:timestamp) (clock
 let event_accept_key (a b srv:principal) (pk_a pk_b ck:bytes) (t:timestamp) (clock_cnt:nat) =
   ("accept_key",[string_to_bytes a;string_to_bytes b;string_to_bytes srv;pk_a;pk_b;ck;nat_to_bytes 0 t;nat_to_bytes 0 clock_cnt])
 
+(* Expected message receive delays in the Denning-Sacco protocol model *)
+
+/// Initiator side second message receive delay
+let recv_msg_2_delay:nat = 2
+/// Responder side third message receive delay
+let recv_msg_3_delay:nat = recv_msg_2_delay + 2
+
 
 /// Format of encrypted/signed message parts
-noeq type encsigval =
-  | SigCertP: p:principal -> pk_p:bytes -> t:timestamp -> encsigval
-  | EncSigCommKey: ck:bytes -> t:timestamp -> encsigval
+noeq type sigval =
+  | CertA: a:principal -> pk_a:bytes -> t:timestamp -> sigval
+  | CertB: b:principal -> pk_b:bytes -> t:timestamp -> sigval
+  | CommKey: ck:bytes -> t:timestamp -> sigval
 
-val parse_encsigval_: sesv:bytes -> result encsigval
+val parse_sigval_: ssv:bytes -> result sigval
 
 
 let ds_key_usages : LC.key_usages = LC.default_key_usages
 
 let can_pke_encrypt (i:nat) s pk m = True
 let can_aead_encrypt i s k m ad = True
-let can_sign i s k m = True
+let can_sign i s k ssv =
+  exists p. LC.get_signkey_label ds_key_usages k == readers [P p] /\
+  (match parse_sigval_ ssv with
+  | Success (CertA a pk_a t) ->
+    (exists b pk_b. did_event_occur_before i p (event_certify a b p pk_a pk_b t 0))
+  | Success (CertB b pk_b t) ->
+    (exists a pk_a. did_event_occur_before i p (event_certify a b p pk_a pk_b t 0))
+  | Success (CommKey ck t) ->
+    exists b. was_rand_generated_before i ck (readers [P p; P b]) (aead_usage "DS.comm_key") /\
+    (exists srv pk_a pk_b. did_event_occur_before i p (event_send_key p b srv pk_a pk_b ck t recv_msg_2_delay))
+  | _ -> False)
 let can_mac i s k m = True
 
 let ds_usage_preds : LC.usage_preds = {
@@ -47,38 +65,62 @@ let ds_global_usage : LC.global_usage = {
   LC.usage_preds = ds_usage_preds;
 }
 
+(* Denning-Sacco specific aliases *)
+
 let msg i l = LC.msg ds_global_usage i l
 let is_msg i b l = LC.is_msg ds_global_usage i b l
 
+let str_to_bytes #i s = LC.string_to_bytes #ds_global_usage #i s
+let nat_to_bytes #i n = LC.nat_to_bytes #ds_global_usage #i 0 n
+let bytes_to_str #i #l b = LC.bytes_to_string #ds_global_usage #i #l b
+let bytes_to_nat #i #l b = LC.bytes_to_nat #ds_global_usage #i #l b
+let concat #i #l b1 b2 = LC.concat #ds_global_usage #i #l b1 b2
+let concat_pub #i b1 b2 = concat #i #public b1 b2
+let split #i #l b = LC.split #ds_global_usage #i #l b
+let split_pub #i b = split #i #public b
 
-let valid_encsigval (i:nat) (esv:encsigval) (l:label) =
-  match esv with
-  | SigCertP p pk_p t -> is_msg i pk_p l
-  | EncSigCommKey ck t -> is_msg i ck l
 
-val serialize_encsigval: i:nat -> esv:encsigval -> l:label{valid_encsigval i esv l} -> sesv:(msg i l)
-val parse_encsigval: #i:nat -> #l:label -> sesv:(msg i l) -> r:(result encsigval)
+let valid_sigval (i:nat) (sv:sigval) (l:label) =
+  match sv with
+  | CertA a pk_a t -> is_msg i pk_a l
+  | CertB b pk_b t -> is_msg i pk_b l
+  | CommKey ck t -> is_msg i ck l
+
+val serialize_sigval: i:nat -> sv:sigval -> l:label{valid_sigval i sv l} -> ssv:(msg i l)
+val parse_sigval: #i:nat -> #l:label -> ssv:(msg i l) -> r:(result sigval)
   {
     match r with
-    | Success esv -> valid_encsigval i esv l
+    | Success sv -> valid_sigval i sv l
     | _ -> True
   }
 
-val parse_encsigval_lemma: #i:nat -> #l:label -> sesv:(msg i l) ->
-  Lemma (parse_encsigval sesv == parse_encsigval_ sesv)
+val parse_sigval_lemma: #i:nat -> #l:label -> ssv:(msg i l) ->
+  Lemma (parse_sigval ssv == parse_sigval_ ssv)
 
-val parse_serialize_encsigval_lemma: i:nat -> esv:encsigval -> l:label ->
-  Lemma (requires (valid_encsigval i esv l))
-        (ensures (parse_encsigval (serialize_encsigval i esv l) == Success esv /\
-                  parse_encsigval_ (serialize_encsigval i esv l) == Success esv))
-        [SMTPat (parse_encsigval (serialize_encsigval i esv l));
-         SMTPat (parse_encsigval_ (serialize_encsigval i esv l))]
+val parse_serialize_sigval_lemma: i:nat -> sv:sigval -> l:label ->
+  Lemma (requires (valid_sigval i sv l))
+        (ensures (parse_sigval (serialize_sigval i sv l) == Success sv /\
+                  parse_sigval_ (serialize_sigval i sv l) == Success sv))
+        [SMTPat (parse_sigval (serialize_sigval i sv l));
+         SMTPat (parse_sigval_ (serialize_sigval i sv l))]
+
+
+/// Create message part to be encrypted, containing the communication key and
+/// a corresponding certificate
+val encval_comm_key: #i:nat -> #l:label -> ser_ck:msg i l -> sig_ck:msg i l -> enc_sig_ck:msg i l
+
+/// Parse decrypted message part, containing the communication key and
+/// a corresponding certificate
+val parse_encval_comm_key: #i:nat -> #l:label -> enc_sig_ck:msg i l -> result (ser_ck:msg i l * sig_ck:msg i l)
+
+val parse_serialize_encval_lemma: #i:nat -> #l:label -> ser_ck:msg i l -> sig_ck:msg i l ->
+  Lemma (parse_encval_comm_key (encval_comm_key ser_ck sig_ck) == Success (ser_ck, sig_ck))
 
 
 noeq type message (i:nat) =
   | Msg1: a:principal -> b:principal -> message i
-  | Msg2: cert_a:msg i public -> cert_b:msg i public -> message i
-  | Msg3: cert_a:msg i public -> cert_b:msg i public -> esv_ck:msg i public -> message i
+  | Msg2: cert_a:msg i public -> sig_cert_a:msg i public -> cert_b:msg i public -> sig_cert_b:msg i public -> message i
+  | Msg3: cert_a:msg i public -> sig_cert_a:msg i public -> cert_b:msg i public -> sig_cert_b:msg i public -> enc_sig_ck:msg i public -> message i
 
 val serialize_msg: i:nat -> m:(message i) -> msg i public
 val parse_msg: #i:nat -> sm:(msg i public) -> r:(result (message i))
