denning-sacco/DS.Protocol.fst
@@ -6,6 +6,10 @@ friend DS.Clock
 
 
 let initiator_send_msg_1 a b srv =
+  // trigger event 'initiate'
+  let event = event_initiate a b srv in
+  trigger_event #ds_preds a event;
+
   // create and send first message
   let now = global_timestamp () in
   let msg1:message now = Msg1 a b in
@@ -23,6 +27,7 @@ let initiator_send_msg_1 a b srv =
 
   (msg1_idx, new_sess_idx)
 
+#push-options "--z3rlimit 50"
 let server_send_msg_2 srv msg1_idx =
   // receive and parse first message
   let (|now,a,ser_msg1|) = receive_i #ds_preds msg1_idx srv in
@@ -35,24 +40,39 @@ let server_send_msg_2 srv msg1_idx =
       let pk_a = get_public_key #ds_preds #now srv a PKE "DS.pke_key" in
       let pk_b = get_public_key #ds_preds #now srv b PKE "DS.pke_key" in
 
+      // initialize clock
+      let t = global_timestamp () in
+      let c_new = clock_new t in
+
+      // trigger event 'certify'
+      let event = event_certify a b srv pk_a pk_b t (clock_get c_new) in
+      trigger_event #ds_preds srv event;
+
       // look up sign key of server and generate sign nonce
+      let now = global_timestamp () in
       let (|_,sigk_srv|) = get_private_key #ds_preds #now srv SIG "DS.sig_key" in
       let (|_,n_sig|) = rand_gen #ds_preds (readers [P srv]) (nonce_usage "SIG_NONCE") in
 
-      // initialize clock
+      // create and sign initiator certificate
+      let cert_a = CertA a pk_a t in
       let now = global_timestamp () in
-      let c_new = clock_new now in
-
-      // create and send second message
-      let esv_sig_cert_a = SigCertP a pk_a now in
-      let ser_cert_a = serialize_encsigval now esv_sig_cert_a public in
+      let ser_cert_a = serialize_sigval now cert_a public in
+      readers_is_injective srv;
+      assert(get_signkey_label ds_key_usages (vk #ds_global_usage #now #(readers [P srv]) sigk_srv) == readers [P srv]);
+      assert(did_event_occur_before now srv (event_certify a b srv pk_a pk_b t 0));
+      parse_serialize_sigval_lemma now cert_a public;
+      assert(can_sign now "DS.sig_key" (vk #ds_global_usage #now #(readers [P srv]) sigk_srv) ser_cert_a);
       let sig_cert_a = sign #ds_global_usage #now #(readers [P srv]) #public sigk_srv n_sig ser_cert_a in
 
-      let esv_sig_cert_b = SigCertP b pk_b now in
-      let ser_cert_b = serialize_encsigval now esv_sig_cert_b public in
+      // create and sign responder certificate
+      let cert_b = CertB b pk_b t in
+      let ser_cert_b = serialize_sigval now cert_b public in
+      parse_serialize_sigval_lemma now cert_b public;
+      assert(can_sign now "DS.sig_key" (vk #ds_global_usage #now #(readers [P srv]) sigk_srv) ser_cert_b);
       let sig_cert_b = sign #ds_global_usage #now #(readers [P srv]) #public sigk_srv n_sig ser_cert_b in
 
-      let msg2 = Msg2 sig_cert_a sig_cert_b in
+      // create and send second message
+      let msg2 = Msg2 ser_cert_a sig_cert_a ser_cert_b sig_cert_b in
       let ser_msg2 = serialize_msg now msg2 in
 
       let (|msg2_idx,c_out|) = SR.send #now c_new srv a ser_msg2 in
@@ -68,3 +88,78 @@ let server_send_msg_2 srv msg1_idx =
       (msg2_idx, new_sess_idx, c_out)
   )
   | _ -> error "[srv_send_m2] wrong message"
+#pop-options
+
+let initiator_send_msg_3 c_in a msg2_idx a_si =
+  // get and parse initiator session
+  let now = global_timestamp () in
+  let (|a_vi,ser_st|) = get_session #ds_preds #now a a_si in
+
+  match parse_session_st ser_st with
+  | Success (InitiatorSentMsg1 b srv) -> (
+    // receive and parse second message
+    let (|now,c_rm2,srv',ser_msg2|) = SR.receive_i msg2_idx c_in a in
+
+    if srv <> srv' then error "[i_send_m3] server stored in session does not match with actual server"
+    else
+      match parse_msg ser_msg2 with
+      | Success (Msg2 cert_a sig_cert_a cert_b sig_cert_b) -> (
+        // look up verification key of server
+        let verk_srv = get_public_key #ds_preds #now a srv SIG "DS.sig_key" in
+
+        // verify initiator and responder certificates
+        if verify #ds_global_usage #now #public #public verk_srv cert_a sig_cert_a then
+          if verify #ds_global_usage #now #public #public verk_srv cert_b sig_cert_b then
+            // parse certificates
+            match (parse_sigval cert_a, parse_sigval cert_b) with
+            | (Success (CertA a pk_a t), Success (CertB b pk_b t')) -> (
+              if t <> t' then error "[i_send_m3] timestamps in initiator and responder certificates do not match"
+              else
+                if clock_lte t recv_msg_2_delay c_rm2 then
+                  // validate public key of initiator
+                  let pk_a' = get_public_key #ds_preds #now a a PKE "DS.pke_key" in
+                  if pk_a <> pk_a' then error "[i_send_m3] wrong initiator public key"
+                  else
+                    // generate communication key
+                    let (|_,ck|) = rand_gen #ds_preds (readers [P a; P b]) (aead_usage "DS.comm_key") in
+
+                    // look up sign key of initiator and generate sign nonce
+                    let (|_,sigk_a|) = get_private_key #ds_preds #now a SIG "DS.sig_key" in
+                    let (|_,n_sig|) = rand_gen #ds_preds (readers [P a]) (nonce_usage "SIG_NONCE") in
+
+                    // generate pke nonce
+                    let (|_,n_pke|) = rand_gen #ds_preds (readers [P a]) (nonce_usage "PKE_NONCE") in
+
+                    // create and sign sigval containing communication key
+                    let sv_comm_key = CommKey ck t in
+                    let now = global_timestamp () in
+                    let ser_comm_key = serialize_sigval now sv_comm_key (readers [P a; P b]) in
+                    let sig_comm_key = sign #ds_global_usage #now #(readers [P a]) #(readers [P a; P b]) sigk_a n_sig ser_comm_key in
+
+                    // create and encrypt encval containing signed sigval with communication key
+                    let ev_comm_key = encval_comm_key ser_comm_key sig_comm_key in
+                    let c_comm_key = pke_enc #ds_global_usage #now #(readers [P a]) pk_b n_pke ev_comm_key in
+
+                    // create and send third message
+                    let msg3 = Msg3 ser_cert_a sig_cert_a ser_cert_b sig_cert_b c_comm_key in
+                    let ser_msg3 = serialize_msg now msg3 in
+
+                    let (|msg3_idx,c_out|) = SR.send #now c_rm2 a b ser_msg3 in
+
+                    // update initiator session
+                    let st_i_sent_m3 = InitiatorSentMsg3 b ck in
+                    let now = global_timestamp () in
+                    let ser_st = serialize_session_st now a a_si a_vi st_i_sent_m3 in
+
+                    update_session #ds_preds #now a a_si a_vi ser_st;
+
+                    (msg3_idx, c_out)
+                else error "[i_send_m3] message has been replayed"
+            )
+            | _ -> error "[i_send_m3] wrong sigvals"
+          else error "[i_send_m3] verification of responder certificate failed"
+        else error "[i_send_m3] verification of initiator certificate failed"
+      )
+      | _ -> error "[i_send_m3] wrong message"
+  )
+  | _ -> error "[i_send_m3] wrong session"
